Time RDTSC several ways

src/hslib/ConcurInterp.hs
@@ -22,7 +22,7 @@ showDebugs :: Bool
 showDebugs = False
 
 timing :: Bool
-timing = False
+timing = True
 
 debugmsg :: String -> IO ()
 debugmsg s = when verbose $ putStrLn s
@@ -101,7 +101,7 @@ run_dcode _ (Debug s n) = do
 run_dcode _ (Rdtsc) = do
   if timing then do
     r <- rdtsc
-    return $ unsafeCoerce r
+    return $ unsafeCoerce (fromIntegral r :: Integer)
   else
     return $ unsafeCoerce (0::Integer)
 run_dcode s (Alloc v) = do
