src/translate.hs
@@ -2,6 +2,7 @@ module Main where
 
 import qualified Interpreter as SeqI
 import qualified ConcurInterp as I
+import qualified OptimisticTranslator
 import TranslateTest
 import ConcurCompile
 import Disk
@@ -28,11 +29,32 @@ measureAction label act = do
   putStrLn $ label ++ show (timePerIter t) ++ " cycles/op"
   return ()
 
+instance Show OptimisticTranslator.OptimisticException where
+  show (OptimisticTranslator.CacheMiss a) = "CacheMiss " ++ show a
+  show OptimisticTranslator.Unsupported = "Unsupported"
+  show OptimisticTranslator.WriteRequired = "WriteRequired"
+
+instance Show a => Show (OptimisticTranslator.Result a) where
+  show (OptimisticTranslator.Success _ v) = "Success " ++ show v
+  show (OptimisticTranslator.Failure e) = "Failure " ++ show e
+
 main :: IO ()
 main = do
   ds <- init_disk "/dev/null"
   cs <- I.newState ds
+  putStrLn "add_tuple results:"
   measureAction "fscq prog " (SeqI.run ds $ add_tuple ((5,6),7) True)
   measureAction "translate " (I.run cs $ add_tuple_concur ((5,6),7) True)
-  measureAction "compiled  " (I.run cs $ compiled_add_tuple ((5,6),7) True)
+  measureAction "compiled  " (I.run cs $ add_tuple_compiled ((5,6),7) True)
   measureAction "raw       " (I.run cs $ add_tuple_concur_raw ((5,6),7) True)
+  putStrLn ""
+  putStrLn "consecutive rdtsc:"
+  t <- SeqI.run ds consecutive_rdtsc
+  putStrLn $ "fscq:      " ++ show t
+  (t, _) <- I.run cs consecutive_rdtsc_concur
+  putStrLn $ "translate: " ++ show t
+  putStrLn ""
+  putStrLn "speed of rdtscs:"
+  measureAction "fscq prog " (SeqI.run ds $ consecutive_rdtsc)
+  measureAction "translate " (I.run cs $ consecutive_rdtsc_concur)
+  measureAction "compiled  " (I.run cs $ consecutive_rdtsc_compiled)
