src/TranslateTest.v
@@ -20,6 +20,17 @@ Definition add_tuple (nums: nat * nat * nat) (b:bool) : prog nat :=
 Definition add_tuple_concur (nums: nat * nat * nat) (b:bool) :=
   translate' (add_tuple nums b) CCLProg.Locked (caches empty_cache empty_cache).
 
+Definition consecutive_rdtsc : prog nat :=
+  t1 <- Rdtsc;
+    t2 <- Rdtsc;
+    Ret (t2-t1).
+
+Definition consecutive_rdtsc_concur :=
+  translate' (consecutive_rdtsc) CCLProg.Locked (caches empty_cache empty_cache).
+
+
+
+(* changes bind notation to build cprog *)
 Import CCLProg.
 
 Definition add_tuple_concur_raw (nums: nat * nat * nat) (b:bool) : cprog _ :=
@@ -33,3 +44,8 @@ Definition add_tuple_concur_raw (nums: nat * nat * nat) (b:bool) : cprog _ :=
     _ <- CacheRead (caches empty_cache empty_cache) 0 CCLProg.Locked;
     Ret 1
   end.
+
+Definition consecutive_rdtsc_concur_raw : cprog nat :=
+  t1 <- Rdtsc;
+    t2 <- Rdtsc;
+    Ret (t2-t1).
